more complicated example Ltacs

examples/Proc.v
@@ -1,87 +1,87 @@
 Require Import MEBI.loader.
 
+Inductive label : Set := | A | B | C.
+
 Inductive action : Set := | ASend | ARecv | BSend | BRecv | CSend | CRecv.
 
-Module NoBranching.
+Inductive term : Set :=
+| trec : term
+| tend : term
+| tfix : term -> term
+| tact : action -> term -> term
+| tpar : term -> term -> term 
+| tseq : term -> term -> term 
+.
 
-  Inductive term : Set :=
-  | trec : term
-  | tend : term
-  | tfix : term -> term
-  | tact : action -> term -> term
-  | tpar : term -> term -> term 
-  | tseq : term -> term -> term 
-  .
+Fixpoint tsubst (t1 : term) (t2 : term) :=
+  match t2 with
+  | trec => t1
+  | tend => tend
+  | tfix t => tfix t
+  | tact a t => tact a (tsubst t1 t)
+  | tpar tl tr => tpar (tsubst t1 tl) (tsubst t1 tr)
+  | tseq t s => tseq t (tsubst t1 s)
+  end.
 
-  Fixpoint tsubst (t1 : term) (t2 : term) :=
-    match t2 with
-    | trec => t1
-    | tend => tend
-    | tfix t => tfix t
-    | tact a t => tact a (tsubst t1 t)
-    | tpar tl tr => tpar (tsubst t1 tl) (tsubst t1 tr)
-    | tseq t s => tseq t (tsubst t1 s)
-    end.
-  
-  (* true: "comm", false: "silent" *)
-  Inductive termLTS : term -> bool -> term -> Prop :=
+(* true: "comm", false: "silent" *)
+Inductive termLTS : term -> option label -> term -> Prop :=
 
-  (* syncrhonous communication, i.e., send/recv in parallel *)
-  | do_senda : forall tl tr,                          (* 0*)
-      termLTS (tpar (tact ASend tl) (tact ARecv tr))
-        true  (tpar tl tr)
+(* syncrhonous communication, i.e., send/recv in parallel *)
+| do_senda : forall tl tr,                          (* 0*)
+    termLTS (tpar (tact ASend tl) (tact ARecv tr))
+      (Some A)  (tpar tl tr)
 
-  | do_sendb : forall tl tr,                          (* 1*)
-      termLTS (tpar (tact BSend tl) (tact BRecv tr))
-        true  (tpar tl tr)
+| do_sendb : forall tl tr,                          (* 1*)
+    termLTS (tpar (tact BSend tl) (tact BRecv tr))
+      (Some B)  (tpar tl tr)
 
-  | do_sendc : forall tl tr,                          (* 2*)
-      termLTS (tpar (tact CSend tl) (tact CRecv tr))
-        true  (tpar tl tr)
+| do_sendc : forall tl tr,                          (* 2*)
+    termLTS (tpar (tact CSend tl) (tact CRecv tr))
+      (Some C)  (tpar tl tr)
 
-  (* asyncrhonous communication, i.e., send/recv in parallel *)
-  (* | do_senda : forall tl tr,                          (* 0*)
-      termLTS (tpar (tact ASend tl) (tact ARecv tr))
-        true  (tpar tl tr)
+(* asyncrhonous communication, i.e., send/recv in parallel *)
+(* | do_senda : forall tl tr,                          (* 0*)
+    termLTS (tpar (tact ASend tl) (tact ARecv tr))
+      true  (tpar tl tr)
 
-  | do_sendb : forall tl tr,                          (* 1*)
-      termLTS (tpar (tact BSend tl) (tact BRecv tr))
-        true  (tpar tl tr)
+| do_sendb : forall tl tr,                          (* 1*)
+    termLTS (tpar (tact BSend tl) (tact BRecv tr))
+      true  (tpar tl tr)
 
-  | do_sendc : forall tl tr,                          (* 2*)
-      termLTS (tpar (tact CSend tl) (tact CRecv tr))
-        true  (tpar tl tr) *)
+| do_sendc : forall tl tr,                          (* 2*)
+    termLTS (tpar (tact CSend tl) (tact CRecv tr))
+      true  (tpar tl tr) *)
 
-  (* non-deterministic parallel step *)
-  (* | do_parl : forall a tl tl' tr,                     (* 3*)
-      termLTS tl a tl' ->
-      termLTS (tpar tl tr) a (tpar tl' tr)
+(* non-deterministic parallel step *)
+(* | do_parl : forall a tl tl' tr,                     (* 3*)
+    termLTS tl a tl' ->
+    termLTS (tpar tl tr) a (tpar tl' tr)
 
-  | do_parr : forall a tl tr tr',                     (* 4*)
-      termLTS tr a tr' ->
-      termLTS (tpar tl tr) a (tpar tl tr') *)
-  | do_seq : forall t t' s a,
-      termLTS t a t' -> termLTS (tseq t s) a (tseq t' s)
+| do_parr : forall a tl tr tr',                     (* 4*)
+    termLTS tr a tr' ->
+    termLTS (tpar tl tr) a (tpar tl tr') *)
+| do_seq : forall t t' s a,
+    termLTS t a t' -> termLTS (tseq t s) a (tseq t' s)
 
-  | do_seq_end : forall s, termLTS (tseq tend s) false s
-  | do_par_end : termLTS (tpar tend tend) false tend
+| do_seq_end : forall s, termLTS (tseq tend s) None s
+| do_par_end : termLTS (tpar tend tend) None tend
 
-  (* These below capture "structural congruence": using "silent" transitions *)
-  | do_fix : forall t,                                (* 5*)
-      termLTS (tfix t) false (tsubst (tfix t) t)
+(* These below capture "structural congruence": using "silent" transitions *)
+| do_fix : forall t,                                (* 5*)
+    termLTS (tfix t) None (tsubst (tfix t) t)
 
-  | do_comm : forall tl tr,                           (* 6*)
-      termLTS (tpar tl tr) false (tpar tr tl)
+| do_comm : forall tl tr,                           (* 6*)
+    termLTS (tpar tl tr) None (tpar tr tl)
 
-  | do_assocl : forall t1 t2 t3,                      (* 7*)
-      termLTS (tpar t1 (tpar t2 t3)) false (tpar (tpar t1 t2) t3)
+| do_assocl : forall t1 t2 t3,                      (* 7*)
+    termLTS (tpar t1 (tpar t2 t3)) None (tpar (tpar t1 t2) t3)
 
-  | do_assocr : forall t1 t2 t3,                      (* 8*)
-      termLTS (tpar (tpar t1 t2) t3) false (tpar t1 (tpar t2 t3))
-  .
-End NoBranching.
+| do_assocr : forall t1 t2 t3,                      (* 8*)
+    termLTS (tpar (tpar t1 t2) t3) None (tpar t1 (tpar t2 t3))
+.
 
-Module WithBranching.
+
+(* Module WithBranching.
   Inductive term : Set :=
   | trec : term
   | tend : term
@@ -163,9 +163,8 @@ Module WithBranching.
       termLTS (tpar p tr) true c ->
       termLTS (tpar p (topt tl tr)) true c *)
   .
-End WithBranching.
+End WithBranching. *)
 
-Import NoBranching.
 (* Import WithBranching. *)
 
 Inductive transitive_closure : term -> Prop :=
@@ -175,110 +174,6 @@ Inductive transitive_closure : term -> Prop :=
 
 | no_step : forall t, transitive_closure t
 .
-
-(*************************************)
-(** Basic: No recursion or branches **)
-(*************************************)
-
-Example proc0_send0 := tact ASend tend. (* empty lts *)
-(* MeBi Show LTS Bounded 150 Of proc0_send0 Using termLTS. *)
-(* MeBi Dump "proc0_send0" LTS Bounded 150 Of proc0_send0 Using termLTS. *)
-
-
-Example proc0_send1a := tpar (tact ASend tend)
-                             (tact ARecv tend).
-(* MeBi Show LTS Bounded 150 Of proc0_send1a Using termLTS. *)
-(* MeBi Dump "proc0_send1a" LTS Bounded 150 Of proc0_send1a Using termLTS. *)
-
-Goal termLTS proc0_send1a true (tpar tend tend).
-  unfold proc0_send1a. eapply do_senda. Qed.
-
-Goal transitive_closure proc0_send1a.
-  unfold proc0_send1a.
-  eapply trans_step. eapply do_senda.
-  constructor.
-Qed.
-
-
-Example proc0_send1b := tpar (tact ARecv tend)
-                             (tact ASend tend).
-(* MeBi Show LTS Bounded 150 Of proc0_send1a Using termLTS. *)
-(* MeBi Dump "proc0_send1b" LTS Bounded 150 Of proc0_send1b Using termLTS. *)
-
-
-Example proc0_send2 := tpar (tact ASend (tact ARecv tend))
-                            (tact ARecv (tact ASend tend)).
-(* MeBi Show LTS Bounded 150 Of proc0_send2 Using termLTS. *)
-(* MeBi Dump "proc0_send2" LTS Bounded 150 Of proc0_send2 Using termLTS. *)
-
-(* Goal transitive_closure proc0_send2.
-  unfold proc0_send2.
-  eapply trans_step. apply do_senda.
-  eapply trans_step. apply do_comm.
-  eapply trans_step. apply do_senda.
-  constructor.
-Qed. *)
-
-
-Example proc0_send3 := tpar (tact ASend (tact BSend tend))
-                            (tact ARecv (tact BRecv tend)).
-(* MeBi Show LTS Bounded 150 Of proc0_send3 Using termLTS. *)
-(* MeBi Dump "proc0_send3" LTS Bounded 150 Of proc0_send3 Using termLTS. *)
-
-
-Example proc0_send4 := tpar (tact BSend (tact ARecv tend))
-                            (tact BRecv (tact ASend tend)).
-(* MeBi Show LTS Bounded 150 Of proc0_send4 Using termLTS. *)
-(* MeBi Dump "proc0_send4" LTS Bounded 150 Of proc0_send4 Using termLTS. *)
-
-
-
-(*************************************)
-(** Recursion ************************)
-(*************************************)
-
-Example proc1_rec1 := tfix trec.
-(* MeBi Show LTS Bounded 150 Of proc1_rec1 Using termLTS. *)
-(* MeBi Dump "proc1_rec1" LTS Bounded 150 Of proc1_rec1 Using termLTS. *)
-
-
-Example proc1_rec2 := tpar (tfix (tact ASend trec))
-                           (tfix (tact ARecv trec)).
-(* MeBi Show LTS Bounded 150 Of proc1_rec2 Using termLTS. *)
-(* MeBi Dump "proc1_rec2" LTS Bounded 150 Of proc1_rec2 Using termLTS. *)
-
-
-Example proc1_rec3 := tpar (tfix (tact ASend (tact BSend trec)))
-                           (tfix (tact ARecv (tact BRecv trec))).
-(* MeBi Show LTS Bounded 150 Of proc1_rec3 Using termLTS. *)
-(* MeBi Dump "proc1_rec3" LTS Bounded 150 Of proc1_rec3 Using termLTS. *)
-
-
-Example proc1_rec4 := tpar (tact ASend (tfix (tact BSend trec)))
-                           (tact ARecv (tfix (tact BRecv trec))).
-(* MeBi Show LTS Bounded 150 Of proc1_rec4 Using termLTS. *)
-(* MeBi Dump "proc1_rec4" LTS Bounded 150 Of proc1_rec4 Using termLTS. *)
-
-
-Example proc1_rec5 := tpar (tfix (tact ASend (tact ASend trec)))
-                           (tfix (tact ARecv trec)).
-(* MeBi Show LTS Bounded 150 Of proc1_rec5 Using termLTS. *)
-(* MeBi Dump "proc1_rec5" LTS Bounded 150 Of proc1_rec5 Using termLTS. *)
-
-
-Example proc1_rec6 := tpar (tact ASend (tact BSend (tfix (tact ASend trec))))
-                           (tpar (tfix (tact ARecv trec))
-                                 (tact BSend tend)).
-(* MeBi Show LTS Bounded 150 Of proc1_rec6 Using termLTS. *)
-(* MeBi Dump "proc1_rec6" LTS Bounded 150 Of proc1_rec6 Using termLTS. *)
-
-
-(* FIXME: grows forever by accumulating [tend]. (need structural equiv.) *)
-Example proc1_rec7 := tfix (tpar (tact ASend (tact BSend trec))
-                                 (tact ARecv (tact BRecv tend))).
-(* MeBi Show LTS Bounded 150 Of proc1_rec7 Using termLTS. *)
-(* MeBi Dump "proc1_rec7" LTS Bounded 150 Of proc1_rec7 Using termLTS. *)
-
 
 
 
@@ -293,7 +188,7 @@ Inductive comp : Set :=
 | cpar : comp -> comp -> comp
 .
 
-Inductive compLTS : comp -> bool -> comp -> Prop :=
+Inductive compLTS : comp -> option label -> comp -> Prop :=
 | do_t : forall a t t',
     termLTS t a t' ->
     compLTS (cterm t) a (cterm t')
@@ -312,237 +207,4 @@ Inductive compLTS : comp -> bool -> comp -> Prop :=
 | do_r_end : forall a l,
     compLTS (cpar l (cterm tend)) a l
 .
-
-(*************************************)
-(** Basic: No recursion or branches **)
-(*************************************)
-
-Example comp1_rec1 := cpar (cterm proc1_rec1) (cterm proc1_rec1).
-(* MeBi Show LTS Bounded 150 Of comp0_send1 Using termLTS compLTS. *)
-(* MeBi Dump "comp1_rec1" LTS Bounded 350 Of comp1_rec1 Using termLTS compLTS. *)
-
-(*************************************)
-(** Recursion ************************)
-(*************************************)
-
-Example comp0_send1 := cpar (cterm proc0_send1a) (cterm proc0_send1b).
-(* MeBi Show LTS Bounded 150 Of comp1_rec1 Using termLTS compLTS. *)
-(* MeBi Dump "comp0_send1" LTS Bounded 350 Of comp0_send1 Using termLTS compLTS. *)
-
-
-
-
-
-
-(****************************************************************************)
-(** Problematic Terms (Branching) *******************************************)
-(** (Requires [tbra] and [topt] ) *******************************************)
-(****************************************************************************)
-(** Issues arise with branching AND recursion *******************************)
-(****************************************************************************)
-
-(* FIXME: these examples grow infinitely without some structural congruence. *)
-
-Inductive bad_term : Set :=
-| bad_trec : bad_term
-| bad_tend : bad_term
-| bad_tfix : bad_term -> bad_term
-| bad_tact : action -> bad_term -> bad_term
-
-(* parallel *)
-| bad_tpar : bad_term -> bad_term -> bad_term
-
-(* active selection/branching *)
-| bad_tbra : bad_term -> bad_term -> bad_term
-
-(* passive option selection/branching *)
-| bad_topt : bad_term -> bad_term -> bad_term
-.
-
-Fixpoint bad_tsubst (t1 : bad_term) (t2 : bad_term) :=
-  match t2 with
-  | bad_trec => t1
-  | bad_tend => bad_tend
-  | bad_tfix t => bad_tfix t
-  | bad_tact a t => bad_tact a (bad_tsubst t1 t)
-  | bad_tpar tl tr => bad_tpar (bad_tsubst t1 tl) (bad_tsubst t1 tr)
-  | bad_tbra tl tr => bad_tbra (bad_tsubst t1 tl) (bad_tsubst t1 tr)
-  | bad_topt tl tr => bad_topt (bad_tsubst t1 tl) (bad_tsubst t1 tr)
-  end.
-
-(* true: "comm", false: "silent" *)
-Inductive bad_termLTS : bad_term -> bool -> bad_term -> Prop :=
-(* syncrhonous communication, i.e., send/recv in parallel *)
-
-| bad_do_senda : forall tl tr,                          (* 0*)
-    bad_termLTS (bad_tpar (bad_tact ASend tl) (bad_tact ARecv tr))
-      true  (bad_tpar tl tr)
-
-| bad_do_sendb : forall tl tr,                          (* 1*)
-    bad_termLTS (bad_tpar (bad_tact BSend tl) (bad_tact BRecv tr))
-      true  (bad_tpar tl tr)
-
-| bad_do_sendc : forall tl tr,                          (* 2*)
-    bad_termLTS (bad_tpar (bad_tact CSend tl) (bad_tact CRecv tr))
-      true  (bad_tpar tl tr)
-
-(* non-deterministic parallel step *)
-| bad_do_parl : forall a tl tl' tr,                     (* 3*)
-    bad_termLTS tl a tl' ->
-    bad_termLTS (bad_tpar tl tr) a (bad_tpar tl' tr)
-
-| bad_do_parr : forall a tl tr tr',                     (* 4*)
-    bad_termLTS tr a tr' ->
-    bad_termLTS (bad_tpar tl tr) a (bad_tpar tl tr')
-
-(* These below capture "structural congruence": using "silent" transitions *)
-| bad_do_fix : forall t,                                (* 5*)
-    bad_termLTS (bad_tfix t) false (bad_tsubst (bad_tfix t) t)
-
-| bad_do_comm : forall tl tr,                           (* 6*)
-    bad_termLTS (bad_tpar tl tr) false (bad_tpar tr tl)
-
-| bad_do_assocl : forall t1 t2 t3,                      (* 7*)
-    bad_termLTS (bad_tpar t1 (bad_tpar t2 t3)) false (bad_tpar (bad_tpar t1 t2) t3)
-
-| bad_do_assocr : forall t1 t2 t3,                      (* 8*)
-    bad_termLTS (bad_tpar (bad_tpar t1 t2) t3) false (bad_tpar t1 (bad_tpar t2 t3))
-
-(* non-deterministic selection between tl and tr *)
-| bad_do_bral : forall a tl tr tl',                     (* 9*)
-    bad_termLTS tl a tl' ->
-    bad_termLTS (bad_tbra tl tr) a tl'
-
-| bad_do_brar : forall a tl tr tr',                     (*10*)
-    bad_termLTS tr a tr' ->
-    bad_termLTS (bad_tbra tl tr) a tr'
-
-(* non-deterministic branch in reaction to ready party p *)
-| bad_do_optl : forall tl tr p c,                       (*11*)
-    bad_termLTS (bad_tpar p tl) true c ->
-    bad_termLTS (bad_tpar p (bad_topt tl tr)) true c
-
-| bad_do_optr : forall tl tr p c,                       (*12*)
-    bad_termLTS (bad_tpar p tr) true c ->
-    bad_termLTS (bad_tpar p (bad_topt tl tr)) true c
-
-
-(* Below are attempts to "clean up" recursive terms. *)
-(* | bad_do_clean :                                        (*13*)
-    bad_termLTS (bad_tpar bad_tend bad_tend) false bad_tend
-
-| bad_do_clean_l : forall tr,                           (*14*)
-    bad_termLTS (bad_tpar bad_tend tr) false tr
-
-| bad_do_clean_r : forall tl,                           (*15*)
-    bad_termLTS (bad_tpar tl bad_tend) false tl *)
-.
-
-
-(*************************************)
-(** Branching, no Recursion **********)
-(*************************************)
-
-Example bad_proc2_bra1 := bad_tbra (bad_tpar (bad_tact ASend bad_tend)
-                                         (bad_tact ARecv bad_tend))
-                               (bad_tpar (bad_tact BSend bad_tend)
-                                         (bad_tact BRecv bad_tend)).
-(* MeBi Show LTS Bounded 150 Of bad_proc2_bra1 Using bad_termLTS. *)
-(* MeBi Dump "bad_proc2_bra1" LTS Bounded 150 Of bad_proc2_bra1 Using bad_termLTS. *)
-
-Example bad_proc2_bra2 :=
-    bad_tbra (bad_tpar (bad_tact ASend (bad_tact BSend bad_tend))
-                       (bad_tact ARecv (bad_tact BRecv bad_tend)))
-             (bad_tpar (bad_tact BSend (bad_tact ASend bad_tend))
-                       (bad_tact BRecv (bad_tact ARecv bad_tend))).
-(* MeBi Show LTS Bounded 150 Of bad_proc2_bra2 Using bad_termLTS. *)
-(* MeBi Dump "bad_bad_proc2_bra2" LTS Bounded 150 Of bad_proc2_bra2 Using bad_termLTS. *)
-
-Example bad_proc2_bra3 :=
-    bad_tbra (bad_tpar (bad_tact ASend (bad_tact BSend bad_tend))
-                       (bad_tact ARecv (bad_tact BRecv bad_tend)))
-             (bad_tbra (bad_tpar (bad_tact BSend (bad_tact CSend bad_tend))
-                                 (bad_tact BRecv (bad_tact CRecv bad_tend)))
-                       (bad_tpar (bad_tact CSend (bad_tact ASend bad_tend))
-                                 (bad_tact CRecv (bad_tact ARecv bad_tend)))).
-(* MeBi Show LTS Bounded 150 Of bad_proc2_bra3 Using bad_termLTS. *)
-(* MeBi Dump "bad_bad_proc2_bra3" LTS Bounded 150 Of bad_proc2_bra3 Using bad_termLTS. *)
-
-
-(*************************************)
-(** Simple Branching and Recursion ***)
-(*************************************)
-
-Example bad_proc3_recbra1 :=
-    bad_tbra (bad_tfix (bad_tpar (bad_tact ASend bad_trec)
-                                 (bad_tact ARecv bad_trec)))
-             (bad_tpar (bad_tact BSend bad_tend)
-                       (bad_tact BRecv bad_tend)).
-(* MeBi Show LTS Bounded 1000 Of bad_proc3_recbra1 Using bad_termLTS. *)
-(* MeBi Dump "bad_proc3_recbra1" LTS Bounded 50 Of bad_proc3_recbra1 Using bad_termLTS. *)
-
-
-Example bad_proc3_recbra2 :=
-    bad_tfix (bad_tbra (bad_tpar (bad_tact ASend bad_trec)
-                                 (bad_tact ARecv bad_trec))
-                       (bad_tpar (bad_tact BSend bad_tend)
-                                 (bad_tact BRecv bad_tend))).
-(* MeBi Show LTS Bounded 1000 Of bad_proc3_recbra2 Using bad_termLTS. *)
-(* MeBi Dump "bad_proc3_recbra2" LTS Bounded 5000 Of bad_proc3_recbra2 Using bad_termLTS. *)
-
-
-Example bad_proc3_recbra3 :=
-    bad_tfix (bad_tbra (bad_tpar (bad_tact ASend bad_trec)
-                                 (bad_tact ARecv bad_trec))
-                       (bad_tpar (bad_tact BSend bad_trec)
-                                 (bad_tact BRecv bad_trec))).
-(* MeBi Show LTS Bounded 1000 Of bad_proc3_recbra3 Using bad_termLTS. *)
-(* MeBi Dump "bad_proc3_recbra3" LTS Bounded 2000 Of bad_proc3_recbra3 Using bad_termLTS. *)
-
-Example bad_proc3_recbra4 :=
-    bad_tbra (bad_tfix (bad_tpar (bad_tact ASend bad_trec)
-                                 (bad_tact ARecv bad_trec)))
-             (bad_tfix (bad_tpar (bad_tact BSend bad_trec)
-                                 (bad_tact BRecv bad_trec))).
-(* MeBi Show LTS Bounded 1000 Of bad_proc3_recbra4 Using bad_termLTS. *)
-(* MeBi Dump "bad_proc3_recbra4" LTS Bounded 2000 Of bad_proc3_recbra4 Using bad_termLTS. *)
-
-(*************************************)
-(** Nested Branching and Recursion ***)
-(*************************************)
-
-
-(* the below example sends [ASend] and then [BSend]. *)
-Example bad_proc1_nestedrec1 :=
-    bad_tfix (bad_tpar ((bad_tact ASend (bad_tact BSend bad_trec)))
-                       (bad_tfix (bad_topt (bad_tact ARecv bad_trec)
-                                           (bad_tact BRecv bad_tend)))).
-
-(* Goal transitive_closure bad_proc1_nestedrec1.
-  unfold bad_proc1_nestedrec1.
-  eapply trans_step. eapply do_fix. simpl.
-  eapply trans_step. eapply do_parr. eapply do_fix. simpl.
-  eapply trans_step. eapply do_optl. eapply do_senda.
-  eapply trans_step. eapply do_parr. eapply do_fix. simpl.
-  eapply trans_step. eapply do_optr. eapply do_sendb.
-  eapply trans_step. eapply do_clean_r.
-  constructor.
-Qed. *)
-
-(* MeBi Show LTS Bounded 150 Of bad_proc1_nestedrec1 Using bad_termLTS. *)
-(* MeBi Dump "bad_proc1_nestedrec1" LTS Bounded 50 Of bad_proc1_nestedrec1 Using bad_termLTS. *)
-
-
-
-
-
-
-
-
-
-(* TODO: would be cool to do first a "FSM minimisation". I believe there are
- many bisimilar states here, where the order (or assoc) of the processes is
- completely irrelevant *)
-(* MeBi Show LTS Bounded 150 Of proc1 Using termLTS. *)
-(* MeBi Dump "proc0" FSM Bounded 150 Of proc1 Using termLTS. *)
 
